\documentclass[hyperref={pdfpagelabels=false}]{beamer}
\setbeamercolor{background canvas}{bg=white}
\usepackage{graphicx,lmodern,subfigure,ulem,color,graphicx,tikz,booktabs,natbib}
\usepackage{mathrsfs}
\usetheme{Warsaw}
%\definecolor{beamer@blendedblue}{rgb}{0.1,0.5,0.1}
%\definecolor{ForestGreen}{RGB}{60, 140, 60}
%\setbeamercolor{structure}{fg=beamer@blendedblue}
\setbeamertemplate{navigation symbols}{}
\setbeamertemplate{footline}[frame number]
\bibliographystyle{chicago}
\newcommand{\spitem}{\vspace{.3cm}\item}
\newcommand{\elas}{$E_{labor}$}
\def \ourFigPath {../../} 

\usetheme[
outer/progressbar=foot,
outer/numbering=none
]{metropolis}



\title{Title}
\author{Marco Brianti\\Vito Cormun}
\institute{Boston College}
\date{March 2019}


\begin{document}
	
	\frame{
		
		
		\maketitle
}




\frame{\frametitle{Equations}
\tiny{
\begin{eqnarray*}
\begin{aligned}
1 &= \beta E \Bigg[ \Bigg( \frac{\{Z_{t}K_{t}^{\alpha} - \eta_1 K_{t-1} - \eta_2 R_t + [ 1 - \gamma_2 Z_{t-1} K_{t-1}^{\alpha}] R_{t-1} (\eta_1K_{t-2} + \eta_2 R_{t-1}) \}}{\{Z_{t+1}K_{t+1}^{\alpha} - \eta_1 K_{t} - \eta_2 R_{t+1} + [ 1 - \gamma_2 Z_t K_t^{\alpha}] R_t (\eta_1 K_{t-1} + \eta_2 R_t) \}}   \Bigg)^{\sigma} \Bigg] [1 + \gamma_2Z_tK_t^{\alpha}]R_t
\end{aligned}
\end{eqnarray*}
}

\begin{eqnarray*}
	K_t = (1 - \delta)K_{t-1} + [ 1 - \gamma_2 (Z_t K_t^{\alpha}) ] (\eta_1 K_{t-1} + \eta_2 R_t )
	\end{eqnarray*}

\begin{eqnarray*}
	Z_t = (1 - \varepsilon_t)Z_{t-1} + \varepsilon_t \lambda R_t
\end{eqnarray*}

\begin{eqnarray*}
\varepsilon_t = \frac{(1 - \rho_t)I_t}{K_t}
\end{eqnarray*}
	
	
}

\frame{\frametitle{Equations}
	
\tiny{
	\begin{eqnarray*}
		\begin{aligned}
			1 &= \beta [1 + \gamma_2 Z_{ss} K_{ss}^{\alpha}]R_{ss}
		\end{aligned}
	\end{eqnarray*}
}

\begin{eqnarray*}
	K_{ss} = (1 - \delta)K_{ss} + [ 1 - \gamma_2 (Z_{ss} K_{ss}^{\alpha}) ] (\eta_1 K_{ss} + \eta_2 R_{ss} )
\end{eqnarray*}

\begin{eqnarray*}
	Z_{ss} = \lambda R_{ss}
\end{eqnarray*}

\begin{eqnarray*}
	\varepsilon_{ss} = \frac{(1 - \rho_{ss})I_{ss}}{K_{ss}}
\end{eqnarray*}
	
		
}


\frame{\frametitle{Equations}
	
	\tiny{
		\begin{eqnarray*}
			\begin{aligned}
				1 &= \beta [1 + \gamma_2 \lambda R_{ss} K_{ss}^{\alpha}]R_{ss} \ \ \Rightarrow \ \ K_{ss} = \bigg(  \frac{1 - \beta R_{ss}}{\gamma_2 \lambda R_{ss}^2}  \bigg)^\frac{1}{\alpha}
			\end{aligned}
		\end{eqnarray*}
	}
	
	\begin{eqnarray*}
		\begin{aligned}
		K_{ss} &= (1 - \delta)K_{ss} + [ 1 - \gamma_2 (\lambda R_{ss} K_{ss}^{\alpha}) ] (\eta_1 K_{ss} + \eta_2 R_{ss} ) \\
		 &\Rightarrow \\
		  	\bigg(  \frac{1 - \beta R_{ss}}{\gamma_2 \lambda R_{ss}^2}  \bigg)^\frac{1}{\alpha} &= (1 - \delta)\bigg(  \frac{1 - \beta R_{ss}}{\gamma_2 \lambda R_{ss}^2}  \bigg)^\frac{1}{\alpha} + \bigg[ 1 - \gamma_2 \bigg( \lambda R_{ss}  \frac{1 - \beta R_{ss}}{\gamma_2 \lambda R_{ss}^2}  \bigg) \bigg] \bigg[ \eta_1 \bigg(  \frac{1 - \beta R_{ss}}{\gamma_2 \lambda R_{ss}^2}  \bigg)^\frac{1}{\alpha} + \eta_2 R_{ss} \bigg]
		  			\end{aligned}
	\end{eqnarray*}
	
	\begin{eqnarray*}
		Z_{ss} = \lambda R_{ss}
	\end{eqnarray*}
	
	\begin{eqnarray*}
		\varepsilon_{ss} = \frac{(1 - \rho_{ss})I_{ss}}{K_{ss}}
	\end{eqnarray*}
	
	
}



\frame{\frametitle{Empirical Strategy}


	
}


\frame{\frametitle{Empirical Results}
	
	
	
}








\frame{\frametitle{Robustness Checks}
	
	
	
}



\frame{\frametitle{Test}
	
	
	
}

\frame{\frametitle{Takeaway}
	
	
	
}


\frame{\frametitle{Model}
	
	
	
}

\frame{\frametitle{Conclusions}
	

	
	
}



\end{document}









\end{document}